# 同余定理
## 若a%m == b%m   则  (a-b)%m == 0
## m|a且m|b   那么m|a+b   ,    m|a-b
证明:
a/m为整数 ， b/m为整数 ， 合并一二式，可得 (a+b)/m =  整数加整数
---
## 证明
设a=mq1+r1,b=mq2+r2,0<=r1,r2<m

∵m|(a-b)

a-b=m(q1-q2)+(r1-r2)

等价于 (a-b)/m - (q1-q2) = (r1- r2)/m

则有m|(r1-r2)

∵0<=r1,r2<m

∴0<=|r1-r2|<m

又∵m|(r1-r2)  即r1-r2=0
∴r1=r2.

---
1. 传递性：若a≡b(mod m)，b≡c(mod m)，则a≡c(mod m)；
2. 同余式相加：若a≡b(mod m)，c≡d(mod m)，则a+c≡b+d(mod m)；
3. 同余式相乘：若a≡b(mod m)，c≡d(mod m)，则ac≡bd(mod m)。
4. 同余式相除：若ac≡bc(mod m),a≡b(mod m/gcd(c,m))
        
        故若c与m互质，有a≡b(mod m)
5. 若a≡b(mod m),则(a,m)=(b,m)
6. 若a≡b(mod m),k|a,k|m,则k|b
---
## 证明
传递性证明：
∵a≡b(mod m)∴m|(a-b) 同理m|(b-c),
∴m|[(a-b)+(b-c)]∴m|(a-c).
故a≡c(mod m).

线性运算：如果a ≡ b (mod m)，c ≡ d (mod m)，那么

(1)a ± c ≡ b ± d (mod m)；

(2)a * c ≡ b * d (mod m)。

证明：

加减
             
(1)∵a≡b(mod m),

∴m|(a-b)

同理 m|(c-d)

∴m|[(a-b)±(c-d)]

∴m|[(a±c)-(b±d)]

∴a ± c ≡ b ± d (mod m)

乘法

(2)∵ac-bd = ac-bc+bc-bd = c(a-b)+b(c-d)

又 m|(a-b) , m|(c-d)

∴m|(ac-bd)

∴a * c ≡ b * d (mod m)